CaseStudies/Velvet/VelvetExamples/EncodeDecodeStr.lean
@@ -1,0 +1,179 @@
+import Auto
+
+import Loom.MonadAlgebras.NonDetT.Extract
+import Loom.MonadAlgebras.WP.Tactic
+import Loom.MonadAlgebras.WP.DoNames'
+
+import CaseStudies.Velvet.Std
+import CaseStudies.TestingUtil
+
+open PartialCorrectness DemonicChoice Lean.Elab.Term.DoNames
+
+set_option auto.smt.trust true
+set_option auto.smt true
+set_option auto.smt.timeout 4
+set_option auto.smt.solver.name "cvc5"
+
+section RunLengthEncoding
+
+structure Encoding where
+  cnt: Nat
+  c: Char
+  deriving Inhabited
+
+variable {velvetString} [arr_inst_int: TArray Char velvetString]
+variable {arrEncoding} [arr_encoding_inst: TArray Encoding arrEncoding]
+
+def get_cnt_sum (l: List Encoding) :=
+  match l with
+  | List.nil => 0
+  | List.cons x xs => x.cnt + get_cnt_sum xs
+  
+lemma get_cnt_sum_hd e l : get_cnt_sum (e::l) = e.cnt + get_cnt_sum l := by
+  conv  => {
+    lhs
+    unfold get_cnt_sum
+  }
+
+
+lemma get_cnt_sum_append l1 l2:  get_cnt_sum (l1 ++ l2) = get_cnt_sum l1 + get_cnt_sum l2 := by
+  induction l1 with
+  | nil => simp; rfl
+  | cons e l1' ih =>
+    simp [ih]
+    grind
+
+@[reducible]
+def is_valid_run_sequence (encoded_str: Array Encoding) := 
+    forall i, ( h: i < encoded_str.size ) -> (encoded_str[i]'h).cnt > 0 
+
+method decodeStr' (encoded_str: Array Encoding) 
+   return (res: Array Char)
+   require is_valid_run_sequence encoded_str
+   ensures (res.size = get_cnt_sum encoded_str.toList)
+     do
+       let mut decoded := Array.replicate 0 'x'
+       let mut i := 0
+       while i < encoded_str.size
+          invariant 0 <= i ∧ i <= encoded_str.size
+          invariant decoded.size = get_cnt_sum (encoded_str.extract 0 i).toList
+          done_with i = encoded_str.size
+          do
+            let elem := encoded_str[i]!
+            let elem_decoded := Array.replicate elem.cnt elem.c
+            decoded :=  decoded ++ elem_decoded
+            i := i + 1
+       return decoded
+
+
+prove_correct decodeStr' by
+  unfold decodeStr'
+  loom_solve
+  · simp[*] at *
+    have : decoded.size = get_cnt_sum (List.take i encoded_str.toList) := by trivial
+    rw [this] at *
+    rw [List.take_succ_eq_append_getElem]
+    rw [get_cnt_sum_append]
+    simp[*]
+    unfold get_cnt_sum
+    rfl
+  · simp[*]; rfl
+  · simp[*]
+
+#eval (decodeStr' #[{cnt:= 10, c:= 'd'}, {cnt := 3, c:= 'e'}, {cnt := 5, c:= 'f'}]).run
+
+def decodeStrLean (encoded_str: Array Encoding) : Array Char := 
+  if h: encoded_str.size > 0 then (
+    let elem := encoded_str[0]
+    (Array.replicate  elem.cnt elem.c) ++ (decodeStrLean (encoded_str.extract 1))
+  )
+  else #[]
+
+#eval (decodeStrLean #[{cnt:= 10, c:= 'd'}, {cnt := 3, c:= 'e'}, {cnt := 5, c:= 'f'}])
+
+lemma decodeStrTriple : forall encoded_str, is_valid_run_sequence encoded_str -> 
+  ( (decodeStrLean encoded_str).size = get_cnt_sum encoded_str.toList)  := by sorry
+
+lemma decodeStrLean_append : forall arr1 arr2, 
+  decodeStrLean (arr1 ++ arr2) = ( decodeStrLean arr1 ) ++ ( decodeStrLean arr2 ) := by sorry
+
+
+
+method encodeStr (str: Array Char) return (res: Array Encoding)
+  ensures is_valid_run_sequence res
+  ensures (decodeStrLean res = str) do
+    let mut encoding : Array Encoding := #[]
+    let mut i := 0
+    while i < str.size 
+    invariant 0 <= i  ∧ i <= str.size
+    invariant decodeStrLean encoding = str.extract 0 i
+    invariant is_valid_run_sequence encoding
+    do
+      let curChar := str[i]!
+      let mut j := i+1
+      while j < str.size ∧ str[j]! == curChar 
+      invariant i < j ∧ j <= str.size
+      invariant (forall k, i <= k ∧ k < j -> str[k]! = curChar )
+      do
+        j := j + 1
+      let cnt := j - i
+      encoding := encoding.push ({cnt:= cnt, c:=curChar})
+      i:=j
+    return encoding
+    
+lemma array_extract_split (arr : Array α) (i j : Nat) :
+    i < j → j ≤ arr.size →
+    arr.extract 0 j = (arr.extract 0 i) ++ (arr.extract i j) := by
+  -- 1. Introduce hypotheses into the context
+  intro h_lt h_le
+  simp[*]
+  grind
+
+lemma array_extract_split_i_j_k (arr : Array α) (i j k: Nat) :
+    i < j -> j < k -> k ≤ arr.size →
+    arr.extract i k = (arr.extract i j) ++ (arr.extract j k) := by
+  -- 1. Introduce hypotheses into the context
+  intro h_lt h_le
+  simp[*]
+  grind
+
+prove_correct encodeStr by
+  unfold encodeStr
+  loom_solve
+  · intros k hik hkj
+    grind
+  · rw [array_extract_split str i j (by assumption) (by assumption)]
+    rw [Array.push_eq_append]
+    rw [decodeStrLean_append]
+    have : decodeStrLean encoding = str.extract 0 i := by trivial
+    rw [this]
+    refine (Array.append_right_inj (str.extract 0 i)).mpr ?_
+    repeat (unfold decodeStrLean ; simp_all)
+    apply Array.ext
+    grind
+    intros l hl hl2
+    rw [Array.size_replicate] at hl
+    simp_all
+    have inv' := invariant_11 (i+l)
+    simp[*] at inv'
+    have : i+l < j  := by trivial
+    have heq := (inv' this)
+    have : i + l < str.size := by
+      grind
+    simp_all
+  · dsimp[is_valid_run_sequence]
+    intros k hk
+    unfold is_valid_run_sequence at *
+    simp_all
+    rw [Array.getElem_push]
+    split_ifs with hk <;> grind
+  · assumption
+  · unfold decodeStrLean 
+    simp[*]
+  · unfold is_valid_run_sequence 
+    simp
+  · simp[*]
+    grind
+  · assumption
+
+end RunLengthEncoding
